add reply function for abs0 and adjust proofs

ds_abs0/ds_abs0_relScript.sml
@@ -3,6 +3,21 @@ open SPI_stateTheory ds_abs0_stateTheory ds_abs0_initTheory ds_abs0_txTheory ds_
 
 val _ = new_theory "ds_abs0_rel";
 
+(* return the received data buffer*)
+val call_back_ds_abs0_def = Define `
+call_back_ds_abs0 (ds_abs0:ds_abs0_state) =
+if ds_abs0.state = abs0_rx_reply then call_back_ds_abs0_rx ds_abs0
+else if ds_abs0.state = abs0_xfer_reply then call_back_ds_abs0_xfer ds_abs0
+else (ds_abs0 with err := T, [])`
+
+val call_back_ds_abs0_state = Define `
+call_back_ds_abs0_state (ds_abs0:ds_abs0_state) =
+let (ds_abs0',l) = call_back_ds_abs0 ds_abs0 in ds_abs0'`
+
+val call_back_ds_abs0_data = Define `
+call_back_ds_abs0_data (ds_abs0:ds_abs0_state) =
+let (ds_abs0',l) = call_back_ds_abs0 ds_abs0 in l`
+
 (* ds_abs0_tr: the state transition relation for ds_abs0 model. *)
 val (ds_abs0_tr_rules, ds_abs0_tr_ind, ds_abs0_tr_cases) = Hol_reln `
 (* call_func labels *)
@@ -14,6 +29,9 @@ ds_abs0_tr ds_abs0 (call_tx buffer) (call_tx_ds_abs0 ds_abs0 buffer)) /\
 ds_abs0_tr ds_abs0 (call_rx length) (call_rx_ds_abs0 ds_abs0 length)) /\
 (!(ds_abs0:ds_abs0_state). (ds_abs0.state = abs0_ready) /\ (buffer <> []) ==>
 ds_abs0_tr ds_abs0 (call_xfer buffer) (call_xfer_ds_abs0 ds_abs0 buffer)) /\
+(!(ds_abs0:ds_abs0_state). (ds_abs0.state = abs0_rx_reply) \/ (ds_abs0.state = abs0_xfer_reply) ==>
+ds_abs0_tr ds_abs0 (call_back (call_back_ds_abs0_data ds_abs0)) 
+(call_back_ds_abs0_state ds_abs0)) /\
 (* TX/RX/XFER *)
 (!(ds_abs0:ds_abs0_state). (ds_abs0.state = abs0_tx) ==>
 ds_abs0_tr ds_abs0 (TX (abs0_tx_op_value ds_abs0)) (abs0_tx_op_state ds_abs0)) /\
@@ -45,6 +63,12 @@ ds_abs0_tr d0 (call_xfer buffer0) d0' ==>
 abs0_global_tr (d0, d1) tau (d0', d1)) /\
 (!d0 d1 buffer1 d1'. 
 ds_abs0_tr d1 (call_xfer buffer1) d1' ==>
+abs0_global_tr (d0, d1) tau (d0, d1')) /\
+(!d0 d1 buffer0 d0'. 
+ds_abs0_tr d0 (call_back buffer0) d0' ==>
+abs0_global_tr (d0, d1) tau (d0', d1)) /\
+(!d0 d1 buffer1 d1'. 
+ds_abs0_tr d1 (call_back buffer1) d1' ==>
 abs0_global_tr (d0, d1) tau (d0, d1')) /\
 (!d0 d1 d0'. ds_abs0_tr d0 tau d0' ==>
 abs0_global_tr (d0, d1) tau (d0', d1)) /\
