ds_abs0/ds_abs0_tauScript.sml
@@ -22,7 +22,9 @@ case ds_abs0.state of
   | abs0_rx_update => abs0_rx_update_tau_op ds_abs0
   | abs0_rx_reading => abs0_rx_reading_tau_op ds_abs0
   | abs0_rx_next => abs0_rx_next_tau_op ds_abs0
+  | abs0_rx_reply => ds_abs0 with err := T
   | abs0_xfer_idle => ds_abs0 with err := T
-  | abs0_xfer_done => abs0_xfer_tau_op ds_abs0`
+  | abs0_xfer_done => abs0_xfer_tau_op ds_abs0
+  | abs0_xfer_reply => ds_abs0 with err := T`
 
 val _ = export_theory();
